abc    b --> c    a ^ (b --> c)    b --> a    (b --> a) ^ c    total
000    1          0                1          0                1
001    1          0                1          1                1
010    0          0                0          0                1
100    1          1                1          0                0
011    1          0                0          0                1
101    1          1                1          1                1
110    0          0                1          0                1
111    1          1                1          1                1

so when a = 1 ^ b = 0 ^ c = 0